Splinter/Betree/PagedBetreeRefinement.i.dfy
@@ -1,0 +1,75 @@
+// Copyright 2018-2021 VMware, Inc., Microsoft Inc., Carnegie Mellon University, ETH Zurich, and University of Washington
+// SPDX-License-Identifier: BSD-2-Clause
+
+include "PagedBetree.i.dfy"
+
+module PagedBetreeRefinement
+{
+  import opened Options
+  import opened KeyType
+  import opened StampedMapMod
+  import TotalKMMapMod
+  import opened ValueMessage
+  import opened MsgHistoryMod
+  import opened LSNMod
+  import opened Sequences
+  import opened PagedBetree
+
+  function INodeAt(betreeNode: BetreeNode, key: Key) : Message
+    requires betreeNode.WF()
+  {
+    BuildQueryReceipt(betreeNode, key).Result()
+  }
+  
+  function INode(betreeNode: BetreeNode) : TotalKMMapMod.TotalKMMap
+    requires betreeNode.WF()
+  {
+    imap key | TotalKMMapMod.AnyKey(key) :: INodeAt(betreeNode, key)
+  }
+
+  function IStampedBetree(stampedBetree: StampedBetree) : StampedMap
+    requires stampedBetree.WF()
+  {
+    StampedMap(INode(stampedBetree.root), stampedBetree.seqEnd)
+  }
+    
+  function I(v: Variables) : StampedMap
+    requires v.WF()
+  {
+    IStampedBetree(v.stampedBetree.PrependMemtable(v.memtable))
+  }
+
+  lemma NoopSteps(v: Variables, v': Variables, lbl: TransitionLabel, step: Step)
+    requires v.WF()
+    requires v'.WF()
+    requires NextStep(v, v', lbl, step)
+    requires !step.PutStep?
+    ensures I(v') == I(v)
+  {
+    match step {
+      case QueryStep(receipt) => {
+        assert Query(v, v', lbl, receipt);
+        assert v' == v;
+        assert I(v') == I(v);
+      }
+      case PutStep() => {
+        assert false;
+      }
+      case QueryEndLsnStep() => {
+        assert I(v') == I(v);
+      }
+      case FreezeAsStep(stampedBetree) => {
+        assert I(v') == I(v);
+      }
+      case InternalSplitStep(_, _) => {
+        assert I(v') == I(v);
+      }
+      case InternalFlushStep(_, _) => {
+        assert I(v') == I(v);
+      }
+      case InternalCompactStep(_, _) => {
+        assert I(v') == I(v);
+      }
+    }
+  }
+}
